Introduce word operation for the core x86 PEXT instruction
The previous PEXT definition resulted in a large and ugly expression.
This is now wrapped up via a general word operation word_condense
which is equipped with an evaluation conversion WORD_CONDENSE_CONV
inside the list extra_word_CONV.

common/misc.ml
@@ -1523,6 +1523,132 @@ extra_word_CONV :=
   WORD_INTERLEAVE_CONV::WORD_SUBDEINTERLEAVE_CONV::(!extra_word_CONV);;
 
 (* ------------------------------------------------------------------------- *)
+(* A basic word operation corresponding to x86's exotic PEXT instruction.    *)
+(* The definition is a bit clumsy and complicated, but as an extra sanity    *)
+(* check and a route to more efficient concrete evaluation we relate it to   *)
+(* a natural-number counterpart defined via recursion on binary digits.      *)
+(* ------------------------------------------------------------------------- *)
+
+let word_condense = define
+ `(word_condense:N word->N word->N word) x y =
+  word(nsum {i | i < dimindex(:N)}
+            (\i. 2 EXP word_popcount(word_and y (word(2 EXP i - 1))) *
+                 bitval(bit i (word_and x y))))`;;
+
+let WORD_CONDENSE_ALT = prove
+ (`!x y:N word.
+    word_condense x y =
+    word(nsum (0..dimindex(:N)-1)
+              (\i. 2 EXP word_popcount(word_and y (word(2 EXP i - 1))) *
+                   bitval(bit i (word_and x y))))`,
+  REWRITE_TAC[word_condense; NUMSEG_LT; DIMINDEX_NONZERO]);;
+
+let num_condense = define
+`num_condense n m =
+  if m = 0 \/ n = 0 then 0
+  else if EVEN m then num_condense (n DIV 2) (m DIV 2)
+  else 2 * num_condense (n DIV 2) (m DIV 2) + bitval(ODD n)`;;
+
+let NUM_CONDENSE_0 = prove
+ (`(!m. num_condense m 0 = 0) /\
+   (!n. num_condense 0 n = 0)`,
+  ONCE_REWRITE_TAC[num_condense] THEN REWRITE_TAC[]);;
+
+let NUM_CONDENSE_CLAUSES = prove
+ (`(!m n. num_condense (2 * n) (2 * m) = num_condense n m) /\
+   (!m n. num_condense (2 * n + 1) (2 * m) = num_condense n m) /\
+   (!m n. num_condense (2 * n) (2 * m + 1) = 2 * num_condense n m) /\
+   (!m n. num_condense (2 * n + 1) (2 * m + 1) = 2 * num_condense n m + 1)`,
+  REPEAT STRIP_TAC THEN GEN_REWRITE_TAC LAND_CONV [num_condense] THEN
+  REWRITE_TAC[ADD_EQ_0; MULT_EQ_0; EVEN_MULT; EVEN_ADD; ODD_ADD; ODD_MULT;
+              BITVAL_CLAUSES; ARITH] THEN
+  REWRITE_TAC[ARITH_RULE `(2 * n) DIV 2 = n /\ (2 * n + 1) DIV 2 = n`] THEN
+  REWRITE_TAC[ADD_CLAUSES] THEN MESON_TAC[NUM_CONDENSE_0; MULT_CLAUSES]);;
+
+let NSUM_CLAUSES_IMAGE = prove
+ (`!f k. nsum {i | i < SUC k} f = f 0 + nsum {i | i < k} (f o SUC)`,
+  GEN_TAC THEN INDUCT_TAC THEN
+  ASM_REWRITE_TAC[NUMSEG_LT; NOT_SUC; NSUM_CLAUSES; ADD_CLAUSES] THEN
+  CONV_TAC NUM_REDUCE_CONV THEN REWRITE_TAC[NSUM_SING; NUMSEG_SING] THEN
+  REWRITE_TAC[SUC_SUB1] THEN
+  SIMP_TAC[NSUM_CLAUSES_LEFT; ARITH_RULE `0 <= SUC n`] THEN
+  AP_TERM_TAC THEN REWRITE_TAC[ADD1; NSUM_OFFSET; o_DEF]);;
+
+let WORD_CONDENSE = prove
+ (`!x y:N word. word_condense x y = word(num_condense (val x) (val y))`,
+  REWRITE_TAC[FORALL_VAL_GEN; word_condense] THEN
+  REWRITE_TAC[BIT_WORD_AND; BIT_MASK_WORD; word_popcount; bits_of_word] THEN
+  SIMP_TAC[BIT_WORD] THEN
+  REWRITE_TAC[TAUT `p /\ (p /\ q) /\ p /\ r <=> (p /\ r) /\ q`] THEN
+  SIMP_TAC[ARITH_RULE `i:num < k ==> (j < k /\ j < i <=> j < i)`] THEN
+  REWRITE_TAC[RIGHT_IMP_FORALL_THM; IMP_IMP] THEN
+  MAP_EVERY X_GEN_TAC [`m:num`; `n:num`] THEN
+  DISCH_TAC THEN AP_TERM_TAC THEN CONV_TAC SYM_CONV THEN POP_ASSUM MP_TAC THEN
+  MAP_EVERY (fun t -> SPEC_TAC(t,t)) [`m:num`;`n:num`] THEN
+  SPEC_TAC(`dimindex(:N)`,`k:num`) THEN INDUCT_TAC THEN
+  SIMP_TAC[EXP; ARITH_RULE `n < 1 <=> n = 0`; CONJUNCT1 LT;
+           NUM_CONDENSE_0; EMPTY_GSPEC; NSUM_CLAUSES] THEN
+  GEN_REWRITE_TAC I [NUM_CASES_BINARY] THEN
+  CONJ_TAC THEN X_GEN_TAC `n:num` THEN
+  GEN_REWRITE_TAC I [NUM_CASES_BINARY] THEN
+  CONJ_TAC THEN X_GEN_TAC `m:num` THEN
+  REWRITE_TAC[ARITH_RULE `2 * m < 2 * n <=> m < n`] THEN
+  REWRITE_TAC[ARITH_RULE `2 * m + 1 < 2 * n <=> m < n`] THEN
+  ASM_SIMP_TAC[NUM_CONDENSE_CLAUSES] THEN POP_ASSUM(K ALL_TAC) THEN
+  ONCE_REWRITE_TAC[SET_RULE
+   `{x | P x /\ Q x} = {x | x IN {y | P y} /\ Q x}`] THEN
+  SIMP_TAC[CARD_EQ_NSUM; FINITE_NUMSEG_LT; FINITE_RESTRICT] THEN
+  REWRITE_TAC[NSUM_RESTRICT_SET] THEN
+  REWRITE_TAC[NSUM_CLAUSES_IMAGE; o_DEF] THEN
+  REWRITE_TAC[EXP; DIV_1; GSYM DIV_DIV] THEN
+  REWRITE_TAC[ARITH_RULE `(2 * n) DIV 2 = n /\ (2 * n + 1) DIV 2 = n`] THEN
+  REWRITE_TAC[ODD_MULT; ODD_ADD; ARITH; BITVAL_CLAUSES; MULT_CLAUSES;
+              ADD_CLAUSES; CONJUNCT1 LT; EMPTY_GSPEC; NSUM_CLAUSES] THEN
+  REWRITE_TAC[CARD_CLAUSES; ARITH_RULE `x + 1 = 1 + y <=> x = y`] THEN
+  REWRITE_TAC[EQ_ADD_RCANCEL; GSYM NSUM_LMUL; EXP_ADD; EXP_1] THEN
+  REWRITE_TAC[MULT_ASSOC]);;
+
+let NUM_CONDENSE_BINARY = prove
+ (`num_condense (NUMERAL(BIT0 n)) (NUMERAL(BIT1 m)) =
+   2 * num_condense (NUMERAL n) (NUMERAL m) /\
+   num_condense (NUMERAL(BIT1 n)) (NUMERAL(BIT1 m)) =
+   2 * num_condense (NUMERAL n) (NUMERAL m) + 1 /\
+   num_condense (NUMERAL(BIT0 n)) (NUMERAL(BIT0 m)) =
+   num_condense (NUMERAL n) (NUMERAL m) /\
+   num_condense (NUMERAL(BIT1 n)) (NUMERAL(BIT0 m)) =
+   num_condense (NUMERAL n) (NUMERAL m)`,
+  REWRITE_TAC[GSYM ADD1; ARITH_RULE `2 = SUC(SUC 0)`] THEN
+  REWRITE_TAC[BIT1; BIT0] THEN
+  ABBREV_TAC `zero = 0` THEN REWRITE_TAC[NUMERAL] THEN
+  FIRST_X_ASSUM(SUBST1_TAC o SYM) THEN
+  REWRITE_TAC[GSYM MULT_2] THEN CONV_TAC NUM_REDUCE_CONV THEN
+  REWRITE_TAC[ARITH_RULE `SUC(2 * n) = 2 * n + 1`; NUM_CONDENSE_CLAUSES]);;
+
+let NUM_CONDENSE_CONV =
+  let [pth_even; pth_odd; pth_base0; pth_base1] =
+    CONJUNCTS NUM_CONDENSE_BINARY in
+  let baseconv = GEN_REWRITE_CONV I [NUM_CONDENSE_0]
+  and evenconv = GEN_REWRITE_CONV I [pth_even]
+  and oddconv = GEN_REWRITE_CONV I [pth_odd]
+  and downconv = GEN_REWRITE_CONV I [pth_base0; pth_base1] in
+  let rec conv tm =
+    (baseconv ORELSEC
+     (downconv THENC conv) ORELSEC
+     (evenconv THENC RAND_CONV conv THENC NUM_MULT_CONV) ORELSEC
+     (oddconv THENC LAND_CONV(RAND_CONV conv THENC NUM_MULT_CONV) THENC
+      NUM_ADD_CONV)) tm in
+  fun tm ->
+    match tm with
+     Comb(Comb(Const("num_condense",_),_),_) -> conv tm
+    | _ -> failwith "NUM_CONDENSE_CONV";;
+
+let WORD_CONDENSE_CONV =
+  GEN_REWRITE_CONV I [WORD_CONDENSE] THENC
+  RAND_CONV(BINOP_CONV WORD_VAL_CONV THENC NUM_CONDENSE_CONV);;
+
+extra_word_CONV := WORD_CONDENSE_CONV::(!extra_word_CONV);;
+
+(* ------------------------------------------------------------------------- *)
 (* A few more lemmas about words.                                            *)
 (* ------------------------------------------------------------------------- *)
 
@@ -1937,7 +2063,7 @@ let UNIFY_REFL_TAC: tactic =
 
 let UNIFY_REFL_TAC_TEST = prove(`?x. 1 = x`, META_EXISTS_TAC THEN UNIFY_REFL_TAC);;
 let UNIFY_REFL_TAC_TEST2 = prove(`?f. y + z = f y z`,
-		META_EXISTS_TAC THEN UNIFY_REFL_TAC);;
+                META_EXISTS_TAC THEN UNIFY_REFL_TAC);;
 
 (* Given `?x1 x2 ... . t` where t is a conjunction of equalities,
    HINT_EXISTS_REFL_TAC infers an assignment for the outermost quantfier x1.
